\documentclass{article}
\usepackage[utf8]{inputenc}

\title{Physically-based Simulation \\ Exercise 1}
\author{ 
    Alexander Lelidis (14-907-562), \\
    Andreas Emch (08-631-384), \\
    Uro\v{s} Te\v{s}i\'{c} (17-950-346)
}
\date{\today}

\usepackage{natbib}
\usepackage{graphicx}

\begin{document}

\maketitle

\section{Analytic solution and results analysis}
\subsection{Analytic solution}
To find the parameters $c_1$ and $c_2$ we use the inital values from the given codebase. The starting position ($t = 0$) is at $y = -1$.
\begin{equation}
    y(t) = c_1 e^{\alpha  t} \cos(\beta t) + c_2 e^{\alpha  t} \sin(\beta t) - L - \frac{mg}{k}
\end{equation}
By  differentiating this equation with respect to t we get.
\begin{equation}
    y'(t) = c_1 e^{\alpha  t} (\alpha \cos(\beta t) - \beta \sin(\beta t) )+ c_2 e^{\alpha  t} (\alpha \sin(\beta t) + \beta \cos(\beta t)) 
\end{equation}
By inserting $t = 0$ and $y_0 = -1$ into (1) we get:
\begin{equation}
    -1 = c_1 e^{\alpha  0} \cos(\beta 0) + c_2 e^{\beta  0} \sin(\beta 0) - L - \frac{mg}{k} 
\end{equation}
\begin{equation}
    -1 = c_1 e^{\alpha  0} - L - \frac{mg}{k} 
\end{equation}
\begin{equation}
    c_1 = -1 + L + \frac{mg}{k}
\end{equation}
To calculate $c_2$ we replace the starting speed with $y'(0) = 0$.
\begin{equation}
    0 = c_1 e^{\alpha  0} (\alpha \cos(\beta 0) - \beta \sin(\beta 0) )+ c_2 e^{\alpha  0} (\alpha \sin(\beta 0) + \beta \cos(\beta 0)) 
\end{equation}
\begin{equation}
    0 = c_1 \alpha \cos(\beta 0) + c_2  \beta \cos(\beta 0)
\end{equation}
\begin{equation}
    0 = c_1 \alpha + c_2  \beta
\end{equation}
\begin{equation}
    c_2 =  \frac{- c_1 \alpha}{  \beta}
\end{equation}
Subsituting $c_1$ to ge the value for $c_2$.
\begin{equation}
    c_2 =  - \frac{ \alpha}{  \beta} (-1 + L + \frac{mg}{k})
\end{equation}

\subsection{Error convergence analysis}
TODO

\subsection{Stability analysis}
TODO

\end{document}
